+

src/ocaml/btree.ml
@@ -2,7 +2,6 @@ let dest_Some = function (Some x) -> x | _ -> failwith "dest_Some"
 
 let option_map f = function Some x -> Some(f x) | _ -> None
 
-
 module Min_size = struct 
   type min_size_t = Small_root_node_or_leaf | Small_node | Small_leaf
 end
@@ -16,8 +15,8 @@ module type CONSTANTS = sig
 end
 
 module type KEY_VALUE_TYPES = sig
-  type key
-  type value_t
+  type key [@@deriving yojson]
+  type value_t [@@deriving yojson]
   val key_ord : key -> key -> int
   val equal_value : value_t -> value_t -> bool (* only for wf checking *)
 end
@@ -46,11 +45,12 @@ module Make = functor (C:CONSTANTS) -> functor (KV:KEY_VALUE_TYPES) -> struct
   module Isa_kv : Our.Key_value_types_t 
     with type key = KV.key and type value_t = KV.value_t 
   = struct
-    type key = KV.key
+    include KV
+(*    type key = KV.key *)
     let key_ord k1 k2 = KV.key_ord k1 k2|>int_to_int
     let equal_keya k1 k2 = KV.key_ord k1 k2 = 0
     let equal_key = Gen_isa.{HOL.equal = equal_keya}
-    type value_t = KV.value_t
+(*    type value_t = KV.value_t *)
     let equal_value_ta = KV.equal_value
     let equal_value_t = Gen_isa.{HOL.equal = equal_value_ta}
   end
@@ -71,18 +71,39 @@ module Make = functor (C:CONSTANTS) -> functor (KV:KEY_VALUE_TYPES) -> struct
     type t = (Tree.tree, unit) Tree_stack.core_t_ext *
           ((Key_value_types.key list * Tree.tree list), unit)
             Tree_stack.core_t_ext list
+
+    let last_state : t option ref = ref None   
+    let last_trans : (t*t option) option ref = ref None
+    let check_state s = (
+      last_state:=Some(s);
+      assert (Find_tree_stack.wellformed_fts s);
+    )
+    let check_trans s s' = (
+      check_state s;
+      match s' with
+      None -> ()
+      | Some t -> (
+          check_state t;
+          last_trans:=Some(s,s');
+          assert (Find_tree_stack.wf_fts_trans s t))
+    )
+
     let mk : key -> M.Tree.tree -> t = fun k0 t -> Find_tree_stack.mk_fts_state k0 t
+
     let step : t -> t option = Find_tree_stack.step_fts
+
     let dest = Find_tree_stack.dest_fts_state
 
     let rec find : key -> t0 -> value_t option = (
       fun k t ->
         let s = ref (mk k t) in
+        let _ = check_state !s in
         let s' = ref(Some(!s)) in
         let _ = 
           while(!s'<>None) do
             s := !s'|>dest_Some;
-            s' := step !s
+            s' := step !s;
+            check_trans !s !s'
           done
         in
         (* !s' is None, so s holds the result *)
@@ -98,19 +119,40 @@ module Make = functor (C:CONSTANTS) -> functor (KV:KEY_VALUE_TYPES) -> struct
 
   module Insert = struct
     type t = Insert_tree_stack.its_state_t
+
+    let last_state : t option ref = ref None   
+    let last_trans : (t*t option) option ref = ref None
+    let check_state s = (
+      last_state:=Some(s);
+      assert (Insert_tree_stack.wellformed_its_state s)
+    )
+    let check_trans x y = (
+      check_state x;
+      match y with
+      None -> ()
+      | Some y' -> (
+          check_state y';
+          last_trans:=Some(x,y);
+          assert (Insert_tree_stack.wf_its_trans x y'))
+    )
+
     let mk : key -> value_t -> M.Tree.tree -> t = 
       fun k v t -> Insert_tree_stack.mk_its_state k v t
+
     let step : t -> t option = Insert_tree_stack.step_its
+
     let dest = Insert_tree_stack.dest_its_state
 
     let rec insert : key -> value_t -> t0 -> t0 = (
       fun k v t ->
         let s = ref (mk k v t) in
+        let _ = check_state !s in
         let s' = ref(Some(!s)) in
         let _ = 
           while(!s'<>None) do
             s := !s'|>dest_Some;
-            s' := step !s
+            s' := step !s;
+            check_trans !s !s';
           done
         in
         (* !s' is None, so s holds the result *)
@@ -118,20 +160,42 @@ module Make = functor (C:CONSTANTS) -> functor (KV:KEY_VALUE_TYPES) -> struct
   end
 
   module Delete = struct
+
     type t = Delete_tree_stack.dts_state_t
+
+    let last_state : t option ref = ref None   
+    let last_trans : (t*t option) option ref = ref None
+    let check_state s = (
+      last_state:=Some(s);
+      assert (Delete_tree_stack.wellformed_dts_state s)
+    )
+    let check_trans x y = (
+      check_state x;
+      match y with
+      None -> ()
+      | Some y' -> (
+          check_state y';
+          last_trans:=Some(x,y);
+          assert (Delete_tree_stack.wf_dts_trans x y'))
+    )
+
     let mk : key -> M.Tree.tree -> t = 
       fun k t -> Delete_tree_stack.mk_dts_state k t
+
     let step : t -> t option = Delete_tree_stack.step_dts
+
     let dest = Delete_tree_stack.dest_dts_state
 
     let rec delete : key -> t0 -> t0 = (
       fun k t ->
         let s = ref (mk k t) in
+        let _ = check_state !s in
         let s' = ref(Some(!s)) in
         let _ = 
           while(!s'<>None) do
             s := !s'|>dest_Some;
-            s' := step !s
+            s' := step !s;
+            check_trans !s !s';
           done
         in
         (* !s' is None, so s holds the result *)
