src/ocaml/bash_env.sh
@@ -12,8 +12,9 @@ root=$(realpath $(dirname $BASH_SOURCE))/../..
  # if using nix, this may not be present
 test -f $root/config.sh && source $root/config.sh
 
-PKGS=""
+PKGS="-package yojson,ppx_deriving_yojson"
 SYNTAX="" # "-syntax camlp4o" # simplify: use for every file
+FLGS="-g"
 
 # 8~"pattern-matching is not exhaustive"; 
 # 11~"this match case is unused";
@@ -21,12 +22,12 @@ SYNTAX="" # "-syntax camlp4o" # simplify: use for every file
 WARN="-w @f@p@u@s@40-8-11-26"
 
 # these include syntax, so should work on all files; may be overridden in ocamlc.sh
-  ocamlc="$DISABLE_BYTE ocamlfind ocamlc   $WARN nums.cma $PKGS $SYNTAX"
-ocamlopt="$DISABLE_NTVE ocamlfind ocamlopt $WARN nums.cmxa $PKGS $SYNTAX"
+  ocamlc="$DISABLE_BYTE ocamlfind ocamlc   $FLGS $WARN nums.cma $PKGS $SYNTAX"
+ocamlopt="$DISABLE_NTVE ocamlfind ocamlopt $FLGS $WARN nums.cmxa $PKGS $SYNTAX"
 ocamldep="ocamlfind ocamldep $PKGS"
 
-mk_cma="$DISABLE_BYTE ocamlfind ocamlc"
-mk_cmxa="$DISABLE_NTVE ocamlfind ocamlopt"
+mk_cma="$DISABLE_BYTE ocamlfind ocamlc $FLGS "
+mk_cmxa="$DISABLE_NTVE ocamlfind ocamlopt $FLGS"
 
 
 mls="gen_isa.ml our.ml btree.ml"
